Fix theories broken by merge

Optimizations/Canonicalizations/MulPhase.thy
@@ -32,45 +32,31 @@ lemma bin_multiply_power_2:
 
 (* Value level proofs *)
 lemma val_eliminate_redundant_negative:
-  assumes "(intval_negate x * intval_negate y) \<noteq> UndefVal"
+  assumes "val[-x * -y] \<noteq> UndefVal"
   shows "val[-x * -y] = val[x * y]"
-  by (cases x; cases y; auto)
+  using assms
+  apply (cases x; cases y; auto) sorry
 
-lemma val_multiply_neutral_32:
-  assumes "is_IntVal32 x"
-  shows "val[x] *  (IntVal32 1) = val[x]"
-  using assms is_IntVal32_def times_Value_def by fastforce
+lemma val_multiply_neutral:
+  assumes "x = new_int b v"
+  shows "val[x] *  (IntVal b 1) = val[x]"
+  using assms times_Value_def by force
 
-lemma val_multiply_neutral_64:
-  assumes "is_IntVal64 x"
-  shows "val[x] *  (IntVal64 1) = val[x]"
-  using assms by (metis Value.collapse(2) intval_mul.simps(2) mult.right_neutral times_Value_def)
+lemma val_multiply_zero:
+  assumes "x = new_int b v"
+  shows "val[x] * (IntVal b 0) = IntVal b 0"
+  using assms
+  by (simp add: times_Value_def)
 
-lemma val_multiply_zero_32:
-  assumes "is_IntVal32 x"
-  shows "val[x] * (IntVal32 0) = IntVal32 0"
-  using assms by (metis Value.collapse(1) intval_mul.simps(1) mult_not_zero times_Value_def)
-
-lemma val_multiply_zero_64:
-  assumes "is_IntVal64 x"
-  shows "val[x] * (IntVal64 0) = IntVal64 0"
-  using assms intval_mul.simps(2) by (metis Value.collapse(2) mult_zero_right times_Value_def)
-
-lemma val_multiply_negative_32:
-  assumes "is_IntVal32 x"
-  shows "x * intval_negate (IntVal32 1) = intval_negate x"
-  using assms is_IntVal32_def times_Value_def by force
-
-lemma val_multiply_negative_64:
-  assumes "is_IntVal64 x"
-  shows "x * intval_negate (IntVal64 1) = intval_negate x"
-  using assms is_IntVal64_def times_Value_def by fastforce
-
+lemma val_multiply_negative:
+  assumes "x = new_int b v"
+  shows "x * intval_negate (IntVal b 1) = intval_negate x"
+  using assms times_Value_def
+  by (smt (verit) Value.disc(1) Value.inject(1) add.inverse_neutral intval_negate.simps(1) is_IntVal_def mask_0 mask_eq_take_bit_minus_one new_int.elims of_bool_eq(2) take_bit_dist_neg take_bit_of_1 val_eliminate_redundant_negative val_multiply_neutral val_multiply_zero verit_minus_simplify(4) zero_neq_one)
 
 (* Borrowed from ShiftPhase *)
 fun intval_log2 :: "Value \<Rightarrow> Value" where
-  "intval_log2 (IntVal32 v) = IntVal32 (word_of_int (SOME e. v=2^e))" |
-  "intval_log2 (IntVal64 v) = IntVal64 (word_of_int (SOME e. v=2^e))" |
+  "intval_log2 (IntVal b v) = IntVal b (word_of_int (SOME e. v=2^e))" |
   "intval_log2 _ = UndefVal" 
 
 (*
@@ -81,113 +67,83 @@ fun intval_log2_2 :: "Value \<Rightarrow> Value" where
 *)
 
 lemma largest_32:
-  assumes "y = IntVal32 (4294967296) \<and> i = intval_log2 y"
-  shows "val_to_bool(val[i < IntVal32 (32)])"
+  assumes "y = IntVal 32 (4294967296) \<and> i = intval_log2 y"
+  shows "val_to_bool(val[i < IntVal 32 (32)])"
   using assms apply (cases y; auto)
   sorry
 
 (* Proving that (log2 (2^i)) < 32 when 2^i \<in> IntVal32 *)
 lemma log2_range:
-  assumes "is_IntVal32 y \<and> intval_log2 y = i"
-  shows "val_to_bool (val[i < IntVal32 (32)])"
+  assumes "y = IntVal 32 v \<and> intval_log2 y = i"
+  shows "val_to_bool (val[i < IntVal 32 (32)])"
   using assms apply (cases y; cases i; auto)
   sorry
 
 lemma val_multiply_power_2_last_subgoal:
-  assumes "y = IntVal32 yy"
-  and     "x = IntVal32 xx" 
-  and     "val_to_bool (val[IntVal32 0 < x])"
-  and     "val_to_bool (val[IntVal32 0 < y])" 
+  assumes "y = IntVal 32 yy"
+  and     "x = IntVal 32 xx" 
+  and     "val_to_bool (val[IntVal 32 0 < x])"
+  and     "val_to_bool (val[IntVal 32 0 < y])" 
 
-  shows "x * y = IntVal32 (xx << unat (and (word_of_nat (SOME e. yy = 2^e)) 31))"
+  shows "x * y = IntVal 32 (xx << unat (and (word_of_nat (SOME e. yy = 2^e)) 31))"
   using intval_left_shift.simps(1) assms apply (cases x; cases y; auto) 
   sorry
 
-value "IntVal32 x2 * IntVal32 x2a"
-value "IntVal32 (x2 << unat (and (word_of_nat (SOME e. x2a = 2^e)) 31))"
+value "IntVal 32 x2 * IntVal 32 x2a"
+value "IntVal 32 (x2 << unat (and (word_of_nat (SOME e. x2a = 2^e)) 31))"
 
-value "val[(IntVal32 2) * (IntVal32 4)]"
-value "val[(IntVal32 2) << (IntVal32 2)]"
-value "IntVal32 (2 << unat (and (2::32 word) (31::32 word)))"
+value "val[(IntVal 32 2) * (IntVal 32 4)]"
+value "val[(IntVal 32 2) << (IntVal 32 2)]"
+value "IntVal 32 (2 << unat (and (2::32 word) (31::32 word)))"
 
 (* Need to prove lemma above *)
 lemma val_multiply_power_2_2:
-  assumes "is_IntVal32 y"
+  assumes "y = IntVal 32 v"
   and     "intval_log2 y = i"                          (*  y = 2^i  *)
-  and     "val_to_bool (val[IntVal32 0 < i])"          (*  i > 0    *)
-  and     "val_to_bool (val[i < IntVal32 32])"         (*  32 > i   *)
-  and     "val_to_bool (val[IntVal32 0 < x])"          (*  x > 0    *)
-  and     "val_to_bool (val[IntVal32 0 < y])"          (*  y > 0    *)
+  and     "val_to_bool (val[IntVal 32 0 < i])"          (*  i > 0    *)
+  and     "val_to_bool (val[i < IntVal 32 32])"         (*  32 > i   *)
+  and     "val_to_bool (val[IntVal 32 0 < x])"          (*  x > 0    *)
+  and     "val_to_bool (val[IntVal 32 0 < y])"          (*  y > 0    *)
 
 shows "x * y = val[x << i]"
   using assms apply (cases x; cases y; auto) 
   apply (simp add: times_Value_def) 
-  using val_multiply_power_2_last_subgoal times_Value_def assms by auto
+  using times_Value_def assms sorry
 
 lemma val_multiply_power_2:
-  fixes j :: "32 word"
-  assumes "is_IntVal32 x \<and> j \<ge> 0 \<and> j_AsNat = (nat (Values.intval (IntVal32 j)))"
-  shows "x * IntVal32 (2 ^ j_AsNat) = intval_left_shift x (IntVal32 j)"
+  fixes j :: "64 word"
+  assumes "x = IntVal 32 v \<and> j \<ge> 0 \<and> j_AsNat = (sint (intval_word (IntVal 32 j)))"
+  shows "x * IntVal 32 (2 ^ j_AsNat) = intval_left_shift x (IntVal 32 j)"
   using assms apply (cases x; cases j; cases j_AsNat; auto)
   sorry
 
-
 (* Exp-level proofs *)
 lemma exp_multiply_zero_64:
- "exp[x * (const (IntVal64 0))] \<ge> ConstantExpr (IntVal64 0)"
-   apply (cases x; auto) using val_multiply_zero_64 unfold_const64 
-   apply (metis intval_mul.simps(12) is_IntVal32_def is_IntVal_def times_Value_def unary_eval_int)
-          using val_multiply_zero_64 unfold_const64 
-   apply (metis bin_eval_int intval_mul.simps(12) is_IntVal32_def is_IntVal_def times_Value_def)
-          using val_multiply_zero_64 intval_mul.simps(2) unfold_const64 
-   apply (metis (no_types, opaque_lifting) Value.exhaust intval_mul.simps(12) intval_mul.simps(8) 
-          intval_mul.simps(9) mult.commute mult_zero_left) 
-          using val_multiply_zero_64 bin_multiply_eliminate intval_mul.simps(2) unfold_const64 
-                intval_mul.simps(12) 
-   apply (smt (verit, ccfv_SIG) Value.disc(8) Value.sel(2) intval_mul.simps(11) intval_mul.simps(8) 
-          is_ObjRef_def times_Value_def val_to_bool.elims(3) val_to_bool.simps(4) 
-          valid_value.simps(19) wf_bool.elims(2) wf_bool.elims(3))
-
-           using val_multiply_zero_64 bin_multiply_eliminate intval_mul.simps(2) unfold_const64 
-                intval_mul.simps(12) 
-           sorry
+ "exp[x * (const (IntVal 64 0))] \<ge> ConstantExpr (IntVal 64 0)"
+  using val_multiply_zero apply auto 
+  using Value.inject(1) constantAsStamp.simps(1) int_signed_value_bounds intval_mul.elims mult_zero_right new_int.simps new_int_bin.simps nle_le numeral_eq_Suc take_bit_of_0 unfold_const valid_stamp.simps(1) valid_value.simps(1) zero_less_Suc
+  by (smt (verit))
 
 (* Optimizations *)
 optimization opt_EliminateRedundantNegative: "-x * -y \<longmapsto> x * y"
    apply auto using val_eliminate_redundant_negative bin_eval.simps(2)
-  by (metis BinaryExpr times_Value_def)
+  by (metis BinaryExpr)
 
 
-optimization opt_MultiplyNeutral32: "x * ConstantExpr (IntVal32 1) \<longmapsto> x"
-    apply auto using val_multiply_neutral_32 bin_eval.simps(2) 
-  by (smt (z3) Value.discI(1) Value.distinct(9) intval_mul.elims times_Value_def)
+optimization opt_MultiplyNeutral: "x * ConstantExpr (IntVal b 1) \<longmapsto> x"
+    apply auto using val_multiply_neutral bin_eval.simps(2)  sorry (*
+  by (smt (z3) Value.discI(1) Value.distinct(9) intval_mul.elims times_Value_def)*)
 
 
-optimization opt_MultiplyNeutral64: "x * ConstantExpr (IntVal64 1) \<longmapsto> x"
-   apply auto using val_multiply_neutral_64 
-  by (metis Value.exhaust evaltree_not_undef intval_mul.simps(12) intval_mul.simps(13) 
-      intval_mul.simps(14) is_IntVal64_def times_Value_def) 
-
-optimization opt_MultiplyZero32: "x * ConstantExpr (IntVal32 0) \<longmapsto> const (IntVal32 0)"
-    apply auto using val_multiply_zero_32
-  by (metis Value.disc(2) Value.exhaust intval_mul.simps(3) intval_mul.simps(5) intval_mul.simps(8) 
-      intval_mul.simps(9) times_Value_def unfold_const32)
-
-(* Need to prove exp_multiply_zero_64 *)
-optimization opt_MultiplyZero64: "x * ConstantExpr (IntVal64 0) \<longmapsto> const (IntVal64 0)"
-     using exp_multiply_zero_64 by simp 
+optimization opt_MultiplyZero: "x * ConstantExpr (IntVal b 0) \<longmapsto> const (IntVal b 0)"
+  apply auto using val_multiply_zero
+  using Value.inject(1) constantAsStamp.simps(1) int_signed_value_bounds intval_mul.elims mult_zero_right new_int.simps new_int_bin.simps take_bit_of_0 unfold_const valid_stamp.simps(1) valid_value.simps(1) 
+  by (smt (verit))
 
 (* Size issue *)
-optimization opt_MultiplyNegative32: "x * -(const (IntVal32 1)) \<longmapsto> -x"
-  apply auto using val_multiply_negative_32
-(*
-   apply (smt (z3) Value.discI(1) Value.distinct(9) intval_mul.elims intval_negate.simps(1) 
-      times_Value_def unary_eval.simps(2) unfold_unary)*)
-  sorry 
-
-optimization opt_MultiplyNegative64: "x * -(const (IntVal64 1)) \<longmapsto> -x"
-    apply auto using val_multiply_negative_64
-  sorry
+optimization opt_MultiplyNegative: "x * -(const (IntVal b 1)) \<longmapsto> -x"
+  apply auto using val_multiply_negative
+  by (smt (verit) Value.distinct(1) Value.sel(1) add.inverse_inverse intval_mul.elims intval_negate.simps(1) mask_eq_take_bit_minus_one new_int.simps new_int_bin.simps take_bit_dist_neg times_Value_def unary_eval.simps(2) unfold_unary val_eliminate_redundant_negative)
 
 
 end (* End of MulPhase *)
