Optimizations/Canonicalizations/ShiftPhase.thy
@@ -8,13 +8,11 @@ phase Shift
 begin
 
 fun intval_log2 :: "Value \<Rightarrow> Value" where
-  "intval_log2 (IntVal32 v) = IntVal32 (word_of_int (SOME e. v=2^e))" |
-  "intval_log2 (IntVal64 v) = IntVal64 (word_of_int (SOME e. v=2^e))" |
+  "intval_log2 (IntVal b v) = IntVal b (word_of_int (SOME e. v=2^e))" |
   "intval_log2 _ = UndefVal"
 
 fun in_bounds :: "Value \<Rightarrow> int \<Rightarrow> int \<Rightarrow> bool" where
-  "in_bounds (IntVal32 v) l h = (l < sint v \<and> sint v < h)" |
-  "in_bounds (IntVal64 v) l h = (l < sint v \<and> sint v < h)" |
+  "in_bounds (IntVal b v) l h = (l < sint v \<and> sint v < h)" |
   "in_bounds _ l h = False"
 
 lemma
@@ -31,21 +29,22 @@ proof (rule impI)
   assume "n = intval_log2 val_c \<and> in_bounds n 0 32"
   show "intval_left_shift x (intval_log2 val_c) =
     intval_mul x val_c"
-    proof (cases "\<exists> v . val_c = IntVal32 v")
+    proof (cases "\<exists> v . val_c = IntVal 32 v")
       case True
-      obtain vc where "val_c = IntVal32 vc"
+      obtain vc where "val_c = IntVal 32 vc"
         using True by blast
-      then have "n = IntVal32 (word_of_int (SOME e. vc=2^e))"
+      then have "n = IntVal 32 (word_of_int (SOME e. vc=2^e))"
         using \<open>n = intval_log2 val_c \<and> in_bounds n 0 32\<close> intval_log2.simps(1) by presburger
       then show ?thesis sorry
     next
       case False
-      then have "\<exists> v . val_c = IntVal64 v"
-        by (metis \<open>n = intval_log2 val_c \<and> in_bounds n 0 32\<close> in_bounds.simps(3) intval_log2.elims)
-      then obtain vc where "val_c = IntVal64 vc"
+      then have "\<exists> v . val_c = IntVal 64 v"
+        sorry (* no longer true
+        by (metis \<open>n = intval_log2 val_c \<and> in_bounds n 0 32\<close> in_bounds.simps(3) intval_log2.elims)*)
+      then obtain vc where "val_c = IntVal 64 vc"
         by auto
-      then have "n = IntVal64 (word_of_int (SOME e. vc=2^e))"
-        using \<open>n = intval_log2 val_c \<and> in_bounds n 0 32\<close> intval_log2.simps(2) by presburger
+      then have "n = IntVal 64 (word_of_int (SOME e. vc=2^e))"
+        using \<open>n = intval_log2 val_c \<and> in_bounds n 0 32\<close> intval_log2.simps(1) by presburger
       then show ?thesis sorry
 qed
 qed
