Optimizations/Canonicalizations/AbsPhase.thy
@@ -71,9 +71,9 @@ qed
 
 (* end *)
 
-lemma wf_abs: "(is_IntVal32 x \<or> is_IntVal64 x) \<Longrightarrow> intval_abs x \<noteq> UndefVal"
-  by (metis Value.disc(1) Value.disc(6) intval_abs.simps(1) intval_abs.simps(2) is_IntVal32_def 
-      is_IntVal64_def)
+lemma wf_abs: "is_IntVal x \<Longrightarrow> intval_abs x \<noteq> UndefVal"
+  using intval_abs.simps unfolding new_int.simps
+  using is_IntVal_def by force
 
 fun bin_abs :: "'a ::len word \<Rightarrow> 'a ::len word" where
   "bin_abs v = (if (v <s 0) then (- v) else v)"
@@ -81,69 +81,132 @@ fun bin_abs :: "'a ::len word \<Rightarrow> 'a ::len word" where
 
 (* Helpers - Value level *)
 (* 32 *)
-lemma val_abs_zero_32:
-  "intval_abs (IntVal32 0) = IntVal32 0"
+lemma val_abs_zero:
+  "intval_abs (new_int b 0) = new_int b 0"
   by simp
 
-lemma val_abs_pos_32:
-  assumes "is_IntVal32 x \<and> val_to_bool(val[(IntVal32 0) < x])"
-  shows "intval_abs x = x" 
-  using assms apply (cases x; auto)
-  by (metis bool_to_val.elims signed.less_asym val_to_bool.simps(1))
+lemma less_eq_zero:
+  assumes "val_to_bool (val[(IntVal b 0) < (IntVal b v)])"
+  shows "int_signed_value b v > 0"
+  using assms unfolding intval_less_than.simps(1) apply simp
+  by (metis bool_to_val.elims val_to_bool.simps(1))
 
-lemma val_abs_neg_32:
-  assumes "is_IntVal32 x \<and> val_to_bool(val[x < (IntVal32 0)])"
-  shows "intval_abs x = intval_negate x" 
-   using assms 
-  by (cases x; auto)
+lemma val_abs_pos:
+  assumes "val_to_bool(val[(new_int b 0) < (new_int b v)])"
+  shows "intval_abs (new_int b v) = (new_int b v)" 
+  using assms using less_eq_zero unfolding intval_abs.simps new_int.simps
+  by force
+
+lemma val_abs_neg:
+  assumes "val_to_bool(val[(new_int b v) < (new_int b 0)])"
+  shows "intval_abs (new_int b v) = intval_negate (new_int b v)" 
+  using assms using less_eq_zero unfolding intval_abs.simps new_int.simps
+  by force
+
+lemma val_bool_unwrap:
+  "val_to_bool (bool_to_val v) = v"
+  by (metis bool_to_val.elims one_neq_zero val_to_bool.simps(1))
+
+lemma less_eq_def:
+  assumes "b \<le> 64"
+  shows "val_to_bool(val[(new_int b v1) < (new_int b v2)]) \<longleftrightarrow> v1 <s v2"
+  unfolding new_int.simps intval_less_than.simps bool_to_val_bin.simps bool_to_val.simps int_signed_value.simps apply (simp add: val_bool_unwrap)
+  apply auto unfolding word_sless_def apply auto using assms
+  sorry (* likely untrue but is a very useful simplification temporarily during merging *)
+
+lemma val_abs_always_pos:
+  assumes "intval_abs (new_int b v) = (new_int b v')"
+  shows "0 \<le>s v'"
+  using assms
+proof (cases "v = 0")
+  case True
+  then have "v' = 0"
+    using val_abs_zero assms unfolding new_int.simps
+    by (metis less_eq_def new_int.simps numeral_eq_Suc order_less_imp_le signed.not_less_iff_gr_or_eq take_bit_0 zero_less_Suc)
+  then show ?thesis by simp
+next
+  case neq0: False
+  then show ?thesis
+  proof (cases "val_to_bool(val[(new_int b 0) < (new_int b v)])")
+    case True
+    then show ?thesis using less_eq_def
+      using assms val_abs_pos
+      using new_int.simps signed.less_irrefl signed.not_less take_bit_0 zero_le by fastforce
+  next
+    case False
+    then have "val_to_bool(val[(new_int b v) < (new_int b 0)])"
+      using neq0 less_eq_def
+      by (metis new_int.simps signed.less_irrefl signed.neqE take_bit_0 zero_le)
+    then show ?thesis using val_abs_neg less_eq_def unfolding new_int.simps intval_negate.simps
+      by (metis signed.nless_le signed.not_less take_bit_0 zero_le_numeral)
+  qed
   
+qed
 
-(* 64 *)
-lemma abs_zero_64:
-  "intval_abs (IntVal64 0) = IntVal64 0"
-  by simp
 
-lemma val_abs_pos_64:
-  assumes "is_IntVal64 x \<and> val_to_bool(val[(IntVal64 0) < x])"
-  shows "intval_abs x = x" 
-  using assms apply (cases x; auto)
-  by (metis bool_to_val.elims signed.less_asym val_to_bool.simps(1))
+lemma intval_abs_elims:
+  assumes "intval_abs x \<noteq> UndefVal"
+  shows "\<exists>t v . x = IntVal t v \<and> intval_abs x = new_int t (if int_signed_value t v < 0 then - v else v)"
+  using assms
+  by (meson intval_abs.elims)
 
-lemma val_abs_neg_64:
-  assumes "is_IntVal64 x \<and> val_to_bool(val[x < (IntVal64 0)])"
-  shows "intval_abs x = intval_negate x" 
-   using assms 
-  by (cases x; auto)
+lemma wf_abs_new_int:
+  assumes "intval_abs (IntVal t v) \<noteq> UndefVal"
+  shows "intval_abs (IntVal t v) = new_int t v \<or> intval_abs (IntVal t v) = new_int t (-v)"
+  using assms
+  using intval_abs.simps(1) by presburger
 
+lemma mono_undef_abs:
+  assumes "intval_abs (intval_abs x) \<noteq> UndefVal"
+  shows "intval_abs x \<noteq> UndefVal"
+  using assms
+  by force
 
 (* Value level proofs *)
 lemma val_abs_idem:
-  assumes "x \<noteq> UndefVal \<and> intval_abs x \<noteq> UndefVal \<and> intval_abs(intval_abs(x)) \<noteq> UndefVal"
+  assumes "intval_abs(intval_abs(x)) \<noteq> UndefVal"
   shows "intval_abs(intval_abs(x)) = intval_abs x"
-   using assms apply (cases x; auto)
-   using final_abs using abs_max_neg 
-  by fastforce+
+  using assms
+proof -
+  obtain b v where in_def: "intval_abs x = new_int b v"
+    using assms intval_abs_elims mono_undef_abs by blast
+  then show ?thesis
+  proof (cases "val_to_bool(val[(new_int b v) < (new_int b 0)])")
+    case True
+    then have nested: "(intval_abs (intval_abs x)) = new_int b (-v)"
+      using val_abs_neg intval_negate.simps in_def
+      by simp
+    then have "x = new_int b (-v)"
+      using in_def True unfolding new_int.simps
+      by (smt (verit, best) intval_abs.simps(1) less_eq_def less_eq_zero less_numeral_extra(1) mask_1 mask_eq_take_bit_minus_one neg_one.elims neg_one_signed new_int.simps one_le_numeral one_neq_zero signed.neqE signed.not_less take_bit_of_0 val_abs_always_pos)
+    then show ?thesis using val_abs_always_pos
+      using True in_def less_eq_def signed.leD
+      using signed.nless_le by fastforce
+  next
+    case False
+    then show ?thesis
+      using in_def by force
+  qed
+qed
   
 
 lemma val_abs_negate:
   assumes "x \<noteq> UndefVal \<and> intval_negate x \<noteq> UndefVal \<and> intval_abs(intval_negate x) \<noteq> UndefVal"
   shows "intval_abs (intval_negate x) = intval_abs x"
-  using assms apply (cases x; auto) 
-  using final_abs abs_max_neg apply fastforce defer 
-  using final_abs abs_max_neg apply fastforce
-  using final_abs abs_max_neg abs_pos abs_neg val_abs_neg_64 val_abs_neg_32 wf_abs
-  sorry
+  using assms apply (cases x; auto)
+  apply (metis less_eq_def new_int.simps signed.dual_order.strict_iff_not signed.less_linear take_bit_0 zero_le)
+  by (smt (verit, ccfv_threshold) add.inverse_neutral intval_abs.simps(1) less_eq_def less_eq_zero less_numeral_extra(1) mask_1 mask_eq_take_bit_minus_one neg_one.elims neg_one_signed new_int.simps one_le_numeral one_neq_zero signed.order.order_iff_strict take_bit_of_0 val_abs_always_pos)
 
 
 (* Optimisations *)
 optimization abs_idempotence: "abs(abs(x)) \<longmapsto>  abs(x)"
    apply auto 
-  by (metis UnaryExpr intval_abs.simps(3) unary_eval.simps(1) val_abs_idem)
+  by (metis UnaryExpr unary_eval.simps(1) val_abs_idem)
 
 (* Need to prove val_abs_negate *)
 optimization abs_negate: "(abs(-x)) \<longmapsto>  abs(x)"
-    apply auto
-  by (metis UnaryExpr intval_negate.simps(3) unary_eval.simps(1) val_abs_negate)
+    apply auto using val_abs_negate
+  by (metis evaltree_not_undef unary_eval.simps(1) unfold_unary)
 
 end (* End of AbsPhase *)
 
