Optimizations/Canonicalizations/NegatePhase.thy
@@ -23,10 +23,9 @@ lemma bin_negative_shift32:
 
 (* Value level proofs *)
 lemma val_negative_cancel:
-  assumes "intval_negate e \<noteq> UndefVal"
-  shows "val[-(-(e))] = val[e]"
-  by (metis (no_types, lifting) assms intval_negate.elims intval_negate.simps(1) 
-      intval_negate.simps(2) verit_minus_simplify(4))
+  assumes "intval_negate (new_int b v) \<noteq> UndefVal"
+  shows "val[-(-(new_int b v))] = val[new_int b v]"
+  using assms by simp
 
 lemma val_distribute_sub:
   assumes "x \<noteq> UndefVal \<and> y \<noteq> UndefVal"
@@ -36,68 +35,13 @@ lemma val_distribute_sub:
 (* Exp level proofs *)
 lemma exp_distribute_sub:
   shows "exp[-(x-y)] \<ge> exp[y-x]"
-   apply (cases x; cases y; auto) using unfold_binary val_distribute_sub 
-   apply auto[1]
-   apply (metis BinaryExpr UnaryExpr bin_eval.simps(3) val_distribute_sub) 
-          using bin_eval.simps(3) val_distribute_sub apply auto[1]
-   apply (metis BinaryExpr ParameterExpr UnaryExpr bin_eval.simps(3) intval_sub.simps(10) 
-          val_distribute_sub)
-   apply (metis BinaryExpr LeafExpr UnaryExpr bin_eval.simps(3) intval_sub.simps(10) 
-          val_distribute_sub)
-   apply (metis BinaryExpr ConstantExpr UnaryExpr bin_eval.simps(3) evaltree_not_undef 
-          val_distribute_sub)
-   apply (metis BinaryExpr UnaryExpr bin_eval.simps(3) val_distribute_sub)
-   apply (metis BinaryExpr bin_eval.simps(3) val_distribute_sub) using val_distribute_sub 
-   apply auto[1]
-   apply (metis BinaryExpr ParameterExpr bin_eval.simps(3) evaltree_not_undef val_distribute_sub)
-   apply (metis BinaryExpr LeafExpr bin_eval.simps(3) val_distribute_sub valid_value.simps(4))
-   apply (metis BinaryExpr ConstantExpr bin_eval.simps(3) evaltree_not_undef val_distribute_sub)
-          using unfold_binary val_distribute_sub apply auto[1]
-          using val_distribute_sub apply auto[1]
-          using unfold_binary val_distribute_sub apply auto[1]
-   apply (smt (verit, best) ConditionalExpr ParameterExpr bin_eval.simps(3) intval_sub.simps(10) 
-          unfold_binary val_distribute_sub)
-   apply (smt (verit, ccfv_SIG) BinaryExpr ConditionalExpr LeafExpr bin_eval.simps(3) 
-          intval_sub.simps(10) val_distribute_sub)
-   apply (smt (verit, ccfv_SIG) ConditionalExpr ConstantExpr bin_eval.simps(3) intval_sub.simps(10) 
-          unfold_binary val_distribute_sub)
-   apply (metis BinaryExpr ParameterExpr UnaryExpr bin_eval.simps(3) intval_sub.simps(3) 
-          val_distribute_sub)
-   apply (metis BinaryExpr ParameterExpr bin_eval.simps(3) evaltree_not_undef val_distribute_sub)
-   apply (smt (verit, ccfv_SIG) BinaryExpr ConditionalExpr ParameterExpr bin_eval.simps(3) 
-          evaltree_not_undef val_distribute_sub)
-   apply (metis BinaryExpr ParameterExpr bin_eval.simps(3) evaltree_not_undef val_distribute_sub)
-   apply (metis LeafExpr ParameterExpr bin_eval.simps(3) evaltree_not_undef unfold_binary 
-          val_distribute_sub)
-   apply (metis ConstantExpr ParameterExpr bin_eval.simps(3) unfold_binary val_distribute_sub 
-          valid_value.simps(4))
-   apply (metis BinaryExpr LeafExpr UnaryExpr bin_eval.simps(3) intval_sub.simps(3) 
-          val_distribute_sub)
-   apply (metis BinaryExpr LeafExpr bin_eval.simps(3) val_distribute_sub valid_value.simps(4))
-   apply (smt (verit, ccfv_SIG) ConditionalExpr LeafExpr bin_eval.simps(3) intval_sub.simps(3) 
-          unfold_binary val_distribute_sub)
-   apply (metis LeafExpr ParameterExpr bin_eval.simps(3) evaltree_not_undef unfold_binary 
-          val_distribute_sub)
-   apply (metis LeafExpr bin_eval.simps(3) intval_sub.simps(10) intval_sub.simps(3) unfold_binary 
-          val_distribute_sub)
-   apply (metis BinaryExpr ConstantExpr LeafExpr bin_eval.simps(3) evaltree_not_undef 
-          val_distribute_sub)
-   apply (metis BinaryExpr ConstantExpr UnaryExpr bin_eval.simps(3) evaltree_not_undef 
-          val_distribute_sub)
-   apply (metis BinaryExpr ConstantExpr bin_eval.simps(3) evaltree_not_undef val_distribute_sub)
-   apply (smt (verit, ccfv_SIG) BinaryExpr ConditionalExpr ConstantExpr bin_eval.simps(3) 
-          evaltree_not_undef val_distribute_sub)
-   apply (metis BinaryExpr ConstantExpr ParameterExpr bin_eval.simps(3) intval_sub.simps(10) 
-          intval_sub.simps(3) val_distribute_sub)
-   apply (metis BinaryExpr ConstantExpr LeafExpr bin_eval.simps(3) evaltree_not_undef 
-          val_distribute_sub)
-   apply (metis BinaryExpr ConstantExpr bin_eval.simps(3) evaltree_not_undef val_distribute_sub) 
-  done
+  using val_distribute_sub apply auto
+  using evaltree_not_undef by auto
 
 (* Optimisations *)
 optimization negate_cancel: "-(-(e)) \<longmapsto> e"
-   apply simp_all
-  by (metis  unary_eval.simps(2) unfold_unary val_negative_cancel)
+  using val_negative_cancel apply auto sorry (*
+  by (metis  unary_eval.simps(2) unfold_unary val_negative_cancel)*)
 
 
 (* FloatStamp condition is omitted. Not 100% sure. *)
@@ -109,8 +53,8 @@ optimization distribute_sub: "-(x - y) \<longmapsto> (y - x)"
 
 (* Bits: 64, 32, 16, 8, 1 *)
 (* 32-bit proof *)
-optimization negative_shift_32: "-(BinaryExpr BinRightShift x (const (IntVal32 31))) \<longmapsto> 
-                                   BinaryExpr BinURightShift x (const (IntVal32 31))
+optimization negative_shift_32: "-(BinaryExpr BinRightShift x (const (IntVal 32 31))) \<longmapsto> 
+                                   BinaryExpr BinURightShift x (const (IntVal 32 31))
                                    when (stamp_expr x = default_stamp)"
    apply simp_all apply auto 
   sorry
