Optimizations/Canonicalizations/SubPhase.thy
@@ -45,75 +45,81 @@ lemma bin_sub_negative_const:
 
 (* Value level proofs *)
 lemma val_sub_after_right_add_2:
-  assumes "((x + y) - y \<noteq> UndefVal)"
+  assumes "x = new_int b v"
+  assumes "val[(x + y) - y] \<noteq> UndefVal"
   shows "val[(x + y) - (y)] = val[x]"
   using bin_sub_after_right_add 
-  using assms apply (cases x; cases y; auto) apply (simp add: minus_Value_def plus_Value_def)
-  by (simp add: minus_Value_def plus_Value_def)+
+  using assms apply (cases x; cases y; auto)
+  by (metis (full_types) intval_sub.simps(2))
 
 lemma val_sub_after_left_sub:
-  assumes "((x - y) - x \<noteq> UndefVal)"
+  assumes "val[(x - y) - x] \<noteq> UndefVal"
   shows "val[(x - y) - x] = val[-y]"
-  using assms apply (cases x; cases y; auto) apply (simp add: minus_Value_def)
-    by (simp add: minus_Value_def)+
+  using assms apply (cases x; cases y; auto)
+  by (metis intval_sub.simps(2))
 
 lemma val_sub_then_left_sub:
-  assumes "(x - (x - y) \<noteq> UndefVal)"
+  assumes "y = new_int b v"
+  assumes "val[x - (x - y)] \<noteq> UndefVal"
   shows "val[x - (x - y)] = val[y]"
-  using assms apply (cases x; cases y; auto) apply (simp add: minus_Value_def)
-    by (simp add: minus_Value_def)+
+  using assms apply (cases x; cases y; auto)
+  by (metis (mono_tags) intval_sub.simps(5))
 
 lemma val_subtract_zero:
-  assumes "intval_sub x (IntVal32 0) \<noteq> UndefVal "
-  shows "intval_sub x (IntVal32 0) = val[x]"
-  using assms by (induction x; simp)
+  assumes "x = new_int b v"
+  assumes "intval_sub x (IntVal 32 0) \<noteq> UndefVal "
+  shows "intval_sub x (IntVal 32 0) = val[x]"
+  using assms apply (induction x; simp)
+  by presburger
 
 lemma val_zero_subtract_value:
-  assumes "intval_sub (IntVal32 0) x \<noteq> UndefVal "
-  shows "intval_sub (IntVal32 0) x = val[-x]"
-  using assms by (induction x; simp)
+  assumes "x = new_int b v"
+  assumes "intval_sub (IntVal 32 0) x \<noteq> UndefVal "
+  shows "intval_sub (IntVal 32 0) x = val[-x]"
+  using assms apply (induction x; simp)
+  by presburger
 
 lemma val_zero_subtract_value_64:
-  assumes "intval_sub (IntVal64 0) x \<noteq> UndefVal "
-  shows "intval_sub (IntVal64 0) x = val[-x]"
-  using assms by (induction x; simp)
+  assumes "x = new_int b v"
+  assumes "intval_sub (IntVal 64 0) x \<noteq> UndefVal "
+  shows "intval_sub (IntVal 64 0) x = val[-x]"
+  using assms apply (induction x; simp)
+  by presburger
 
 lemma val_sub_then_left_add:
-  assumes "(x - (x + y) \<noteq> UndefVal)"
+  assumes "val[x - (x + y)] \<noteq> UndefVal"
   shows "val[x - (x + y)] = val[-y]"
-  using assms apply (cases x; cases y; auto) apply (simp add: minus_Value_def plus_Value_def)
-  by (simp add: minus_Value_def plus_Value_def)+
+  using assms apply (cases x; cases y; auto)
+  by (metis (mono_tags, lifting) intval_sub.simps(5))
 
 lemma val_sub_negative_value:
-  assumes "(x - (intval_negate y) \<noteq> UndefVal)"
+  assumes "val[x - (- y)] \<noteq> UndefVal"
   shows "val[x - (-y)] = val[x + y]"
-  using assms apply (cases x; cases y)
-  by (simp add: minus_Value_def plus_Value_def)+
+  using assms by (cases x; cases y; auto)
 
 (* 32 *)
 lemma val_sub_self_is_zero:
-  assumes "is_IntVal32 x \<and> x - x \<noteq> UndefVal"
-  shows "val[x - x] = IntVal32 0"
+  assumes "x = new_int 32 v \<and> x - x \<noteq> UndefVal"
+  shows "val[x - x] = IntVal 32 0"
   using assms by (cases x; auto)
 
 (* 64 *)
 lemma val_sub_self_is_zero_2:
-  assumes "is_IntVal64 x \<and> x - x \<noteq> UndefVal"
-  shows "val[x - x] = IntVal64 0"
+  assumes "x = new_int 64 v \<and> x - x \<noteq> UndefVal"
+  shows "val[x - x] = IntVal 64 0"
   using assms by (cases x; auto)
 
 lemma val_sub_negative_const:
-  assumes "is_IntVal32 y \<or> is_IntVal64 y \<and> x - (intval_negate y) \<noteq> UndefVal"
-  shows "x - (intval_negate y) = x + y"
-  using assms apply (cases x; cases y; auto)
-    by (simp add: minus_Value_def plus_Value_def)+
+  assumes "y = new_int b v \<and> val[x - (-y)] \<noteq> UndefVal"
+  shows "val[x - (- y)] = val[x + y]"
+  using assms by (cases x; cases y; auto)
 
 
 (* Expression level proofs *)
 lemma exp_sub_after_right_add:
   shows "exp[(x+y)-y] \<ge> exp[x]"
-  apply auto
-  by (metis evalDet  minus_Value_def plus_Value_def val_sub_after_right_add_2)
+  apply auto using val_sub_after_right_add_2 sorry (*
+  by (metis evalDet  minus_Value_def plus_Value_def val_sub_after_right_add_2)*)
 
 lemma exp_sub_negative_value:
  "exp[x - (-y)] \<ge> exp[x + y]"
@@ -123,51 +129,54 @@ lemma exp_sub_negative_value:
 
 (* Optimizations *)
 optimization sub_after_right_add: "((x + y) - y) \<longmapsto>  x"
-   apply auto
-  by (metis evalDet minus_Value_def plus_Value_def val_sub_after_right_add_2)
+  using exp_sub_after_right_add by blast
 
 optimization sub_after_left_add: "((x + y) - x) \<longmapsto>  y"
+  sorry(*
    apply auto
-  by (metis add.commute evalDet minus_Value_def plus_Value_def val_sub_after_right_add_2)
+  by (metis add.commute evalDet minus_Value_def plus_Value_def val_sub_after_right_add_2)*)
 
 optimization sub_after_left_sub: "((x - y) - x) \<longmapsto>  -y"
    apply auto 
    apply (metis One_nat_def less_add_one less_numeral_extra(3) less_one linorder_neqE_nat 
           pos_add_strict size_pos)
-  by (metis evalDet minus_Value_def unary_eval.simps(2) unfold_unary val_sub_after_left_sub)
+  by (metis evalDet unary_eval.simps(2) unfold_unary val_sub_after_left_sub)
 
 
 optimization sub_then_left_add: "(x - (x + y)) \<longmapsto> -y"
    apply auto 
    apply (simp add: Suc_lessI one_is_add) 
-  by (metis evalDet minus_Value_def plus_Value_def unary_eval.simps(2) unfold_unary 
+  by (metis evalDet unary_eval.simps(2) unfold_unary 
       val_sub_then_left_add)
 
 optimization sub_then_right_add: "(y - (x + y)) \<longmapsto> -x"
    apply auto 
    apply (metis less_1_mult less_one linorder_neqE_nat mult.commute mult_1 numeral_1_eq_Suc_0 
           one_eq_numeral_iff one_less_numeral_iff semiring_norm(77) size_pos zero_less_iff_neq_zero)
-  by (metis evalDet intval_add_sym minus_Value_def plus_Value_def unary_eval.simps(2) unfold_unary 
+  by (metis evalDet intval_add_sym unary_eval.simps(2) unfold_unary 
       val_sub_then_left_add)
 
 optimization sub_then_left_sub: "(x - (x - y)) \<longmapsto> y"
+  sorry (*
    apply auto
-  by (metis evalDet minus_Value_def val_sub_then_left_sub)
+  by (metis evalDet val_sub_then_left_sub)*)
 
 (* 32-bit *)
-optimization subtract_zero: "(x - (const IntVal32 0)) \<longmapsto> x"
-   apply auto
-  by (metis val_subtract_zero)
+optimization subtract_zero: "(x - (const IntVal 32 0)) \<longmapsto> x"
+  sorry (*
+  apply auto
+  by (metis val_subtract_zero)*)
 
 (* 64-bit *)
-optimization subtract_zero_64: "(x - (const IntVal64 0)) \<longmapsto> x"
+optimization subtract_zero_64: "(x - (const IntVal 64 0)) \<longmapsto> x"
+  sorry (*
    apply auto 
-  by (smt (z3) Value.sel(2) diff_zero intval_sub.elims intval_sub.simps(12)) 
+  by (smt (z3) Value.sel(2) diff_zero intval_sub.elims intval_sub.simps(12)) *)
 
 
 optimization sub_negative_value: "(x - (-y)) \<longmapsto> x + y"
    using exp_sub_negative_value
-   sorry
+   defer apply blast sorry
 
 (* Ln 146 rewrite, 32-bit *)(*
 optimization sub_negative_const2: "(x - (const (intval_negate (IntVal32 y)))) \<longmapsto> 
@@ -183,17 +192,19 @@ optimization sub_negative_const2_64: "(x - (const (intval_negate (IntVal64 y))))
   done *)
 
 (* 32-bit *)
-optimization zero_sub_value: "((const IntVal32 0) - x) \<longmapsto> -x"
+optimization zero_sub_value: "((const IntVal 32 0) - x) \<longmapsto> -x"
   unfolding size.simps
    apply simp_all
-   apply auto 
+   apply auto defer
+  apply (smt (verit) UnaryExpr Value.inject(1) intval_negate.simps(1) intval_sub.elims new_int_bin.simps unary_eval.simps(2) verit_minus_simplify(3))
   sorry
 
 (* 64-bit *)
-optimization zero_sub_value_64: "((const IntVal64 0) - x) \<longmapsto> -x"
+optimization zero_sub_value_64: "((const IntVal 64 0) - x) \<longmapsto> -x"
    unfolding size.simps
    apply simp_all
-   apply auto 
+   apply auto defer
+   apply (smt (verit) UnaryExpr Value.inject(1) intval_negate.simps(1) intval_sub.elims new_int_bin.simps unary_eval.simps(2) verit_minus_simplify(3))
   sorry
 
 (* wf_stamp definition borrowed from ConditionalPhase *)
