Optimizations/Canonicalizations/TacticSolving.thy
@@ -100,7 +100,7 @@ optimization distribute_sub: "-(x-y) \<longmapsto> (y-x)"
   using unfold_binary unfold_unary by auto
 
 lemma val_xor_self_is_false:
-  assumes "is_IntVal32 x"
+  assumes "x = IntVal 32 v"
   shows "val[x \<oplus> x] \<approx> val[false]"
   apply simp using assms by (cases x; auto)
 
@@ -114,29 +114,34 @@ lemma exp_xor_self_is_false:
   shows "exp[x \<oplus> x] >= exp[false]"
   unfolding le_expr_def using assms unfolding wf_stamp_def
   using val_xor_self_is_false evaltree_not_undef
-  by (metis BinaryExprE Value.disc(2) bin_eval.simps(6) evalDet unfold_const32 valid_int32 well_formed_equal_defn)
+  by (smt (z3) bin_eval.simps(6) bin_eval_new_int constantAsStamp.simps(1) evalDet int_signed_value_bounds new_int.simps new_int_take_bits unfold_binary unfold_const valid_int valid_stamp.simps(1) valid_value.simps(1) well_formed_equal_defn)
+
+
 
 lemma OrInverseVal:
-  assumes "is_IntVal32 n"
-  shows "val[n | ~n] \<approx> IntVal32 (-1)"
-  apply simp using assms using word_or_not by (cases n; auto)
+  assumes "n = IntVal 32 v"
+  shows "val[n | ~n] \<approx> new_int 32 (-1)"
+  apply simp using assms using word_or_not apply (cases n; auto) using take_bit_or
+  by (metis bit.disj_cancel_right mask_eq_take_bit_minus_one)
 
-optimization OrInverse: "exp[n | ~n] \<longmapsto> (const (IntVal32 (not 0)))
+optimization OrInverse: "exp[n | ~n] \<longmapsto> (const (new_int 32 (not 0)))
                         when (stamp_expr n = IntegerStamp 32 l h \<and> wf_stamp n)"
   unfolding size.simps apply (simp add: Suc_lessI)
-  apply auto using OrInverseVal
-  by (metis evalDet is_IntVal32_def unfold_const32 valid_int32 well_formed_equal_defn wf_stamp_def)
+  apply auto using OrInverseVal unfolding wf_stamp_def
+  by (smt (z3) constantAsStamp.simps(1) evalDet int_signed_value_bounds mask_eq_take_bit_minus_one new_int.elims new_int_take_bits unfold_const valid_int valid_stamp.simps(1) valid_value.simps(1) well_formed_equal_defn)
+
 
 lemma XorInverseVal:
-  assumes "is_IntVal32 n"
-  shows "val[n \<oplus> ~n] \<approx> IntVal32 (-1)"
-  apply simp using assms using word_or_not by (cases n; auto)
+  assumes "n = IntVal 32 v"
+  shows "val[n \<oplus> ~n] \<approx> new_int 32 (-1)"
+  apply simp using assms using word_or_not apply (cases n; auto)
+  by (metis (no_types, opaque_lifting) bit.compl_zero bit.xor_compl_right bit.xor_self mask_eq_take_bit_minus_one take_bit_xor)
 
-optimization XorInverse: "exp[n \<oplus> ~n] \<longmapsto> (const (IntVal32 (not 0)))
+optimization XorInverse: "exp[n \<oplus> ~n] \<longmapsto> (const (new_int 32 (not 0)))
                         when (stamp_expr n = IntegerStamp 32 l h \<and> wf_stamp n)"
   unfolding size.simps apply (simp add: Suc_lessI)
   apply auto using XorInverseVal
-  by (metis Value.disc(2) evalDet unfold_const32 valid_int32 well_formed_equal_defn wf_stamp_def)
+  by (smt (verit) constantAsStamp.simps(1) evalDet int_signed_value_bounds intval_xor.elims mask_eq_take_bit_minus_one new_int.elims new_int_take_bits unfold_const valid_stamp.simps(1) valid_value.simps(1) well_formed_equal_defn wf_stamp_def)
 
 
 end
